\subsection{Question 1}

From the continuous plant

\begin{align*}
  \dot{x}(t) &= Ax(t) + Bu(t) \\
        y(t) &= Cx(t)
\end{align*}

and the facts that $A=0, B=1, \tau \in [0,h]$ we can derive the equation for the
discretized state

\begin{align*}
  x[(k+1)h] &= \Phi x[kh] + \Gamma_0 u[kh] + \Gamma_1 u[(k-1)h] \\
  x[(k+1)h] &= x[kh] + (h-\tau)u[kh] + \tau u[(k-1)h] \\
\end{align*}

where

\begin{align*}
  \Phi      &= e^{Ah} = 1 \\
  \Gamma_0  &= \int_{0}^{h-\tau} e^{As} ds B = h-\tau \\
  \Gamma_1  &= e^{A(h-t)} \int_{0}^{\tau} e^{As} ds B = \tau
\end{align*}

Due to the additional delayed input term $u[(k-1)h]$, the system's state is
augmented and is now considered as the vector

\begin{align*}
  s =
  \begin{bmatrix}
    x[kh] \\
    u[(k-1)h]
  \end{bmatrix}
\end{align*}

Considering the fact that $u[kh] = -K x[kh]$, the equations of the closed-loop
system thus become

\begin{align*}
  \begin{bmatrix}
    x[(k+1)h] \\
    u[kh]
  \end{bmatrix}
  =
  \begin{bmatrix}
    \Phi - \Gamma_0 K & \Gamma_1 \\
    -K                & 0 \\
  \end{bmatrix}
  \begin{bmatrix}
    x[kh] \\
    u[(k-1)h]
  \end{bmatrix}
\end{align*}

or

\begin{align*}
  \begin{bmatrix}
    x[(k+1)h] \\
    u[kh]
  \end{bmatrix}
  =
  \begin{bmatrix}
    1 - (h-\tau)K & \tau \\
    -K            & 0 \\
  \end{bmatrix}
  \begin{bmatrix}
    x[kh] \\
    u[(k-1)h]
  \end{bmatrix}
\end{align*}
